define riscv example program boundaries centrally instead of hardcoding address constants

examples/riscv/common/bir_symbLib.sig
@@ -3,16 +3,17 @@ sig
 
   include Abbrev;
 
-  val mem_addrs_prog_disj_tm : string -> term;
+  val mem_addrs_prog_disj_bir_tm : string -> term;
 
-  val mem_addrs_aligned_prog_disj_tm : string -> term;
-  val mem_addrs_aligned_prog_disj_riscv_tm : term -> term;
+  val mem_addrs_aligned_prog_disj_bir_tm : string -> term;
 
-  val pre_vals_reg_tm : string -> string -> term;
+  val mem_addrs_aligned_prog_disj_riscv_tm : string -> term;
 
-  val pre_vals_mem_reg_tm : string -> string -> string -> term;
+  val pre_vals_reg_bir_tm : string -> string -> term;
 
-  val pre_vals_tm : string -> string -> string -> string -> term;
+  val pre_vals_mem_reg_bir_tm : string -> string -> string -> term;
+
+  val pre_vals_bir_tm : string -> string -> string -> string -> term;
 
   val bir_symb_analysis : term -> term -> term list -> term -> term -> thm;
 
