examples/riscv/aes/aes_specScript.sml
@@ -14,6 +14,22 @@ open aesTheory;
 
 val _ = new_theory "aes_spec";
 
+(* ------------------ *)
+(* Program boundaries *)
+(* ------------------ *)
+
+Definition aes_init_addr_def:
+ aes_init_addr : word64 = 0x088w
+End
+
+Definition aes_end_addr_def:
+ aes_end_addr : word64 = 0x208w
+End
+
+(* -------------- *)
+(* BSPEC contract *)
+(* -------------- *)
+
 val registervars_tm = ``[
     BVar "x31" (BType_Imm Bit64);
     BVar "x30" (BType_Imm Bit64);
@@ -42,11 +58,14 @@ Definition bir_aes_registervars_def:
  bir_aes_registervars = ^registervars_tm
 End
 
-val bir_aes_pre_tm = bslSyntax.bandl (List.map (mem_addrs_aligned_prog_disj_tm o stringSyntax.fromHOLstring o fst o bir_envSyntax.dest_BVar) ((fst o listSyntax.dest_list) registervars_tm));
+val bspec_aes_pre_tm = bslSyntax.bandl
+ (List.map (mem_addrs_aligned_prog_disj_bir_tm o
+   stringSyntax.fromHOLstring o fst o bir_envSyntax.dest_BVar)
+  ((fst o listSyntax.dest_list) registervars_tm));
 
-Definition bir_aes_pre_def:
-  bir_aes_pre : bir_exp_t =
-   ^bir_aes_pre_tm
+Definition bspec_aes_pre_def:
+  bspec_aes_pre : bir_exp_t =
+   ^bspec_aes_pre_tm
 End
 
 val _ = export_theory ();
