examples/riscv/aes/aes_symb_execScript.sml
@@ -15,9 +15,7 @@ val _ = new_theory "aes_symb_exec";
 val registervars_tm = (snd o dest_eq o concl) bir_aes_registervars_def;
 
 Definition aes_prog_vars_def:
-  aes_prog_vars = 
-    (BVar "MEM8" (BType_Mem Bit64 Bit8))
-    ::(^registervars_tm)
+  aes_prog_vars = (BVar "MEM8" (BType_Mem Bit64 Bit8))::(^registervars_tm)
 End
 
 Definition aes_birenvtyl_def:
@@ -38,17 +36,20 @@ QED
 
 Theorem aes_bsysprecond_thm =
  (computeLib.RESTR_EVAL_CONV [``birs_eval_exp``] THENC birs_stepLib.birs_eval_exp_CONV)
- ``mk_bsysprecond bir_aes_pre aes_birenvtyl``;
+ ``mk_bsysprecond bspec_aes_pre aes_birenvtyl``;
 
 (* ----------------------- *)
 (* Symbolic analysis setup *)
 (* ----------------------- *)
 
 val bprog_tm = (snd o dest_eq o concl) bir_aes_prog_def;
+val init_addr_tm = (snd o dest_eq o concl) aes_init_addr_def;
+val end_addr_tm = (snd o dest_eq o concl) aes_end_addr_def;
 
-val birs_state_init_lbl = (snd o dest_eq o concl o EVAL) ``bir_block_pc (BL_Address (Imm64 0x088w))``;
-
-val birs_stop_lbls = [(snd o dest_eq o concl o EVAL) ``bir_block_pc (BL_Address (Imm64 0x208w))``];
+val birs_state_init_lbl = (snd o dest_eq o concl o EVAL)
+ ``bir_block_pc (BL_Address (Imm64 ^init_addr_tm))``;
+val birs_state_end_lbls = [(snd o dest_eq o concl o EVAL)
+ ``bir_block_pc (BL_Address (Imm64 ^end_addr_tm))``];
 
 val bprog_envtyl = (fst o dest_eq o concl) aes_birenvtyl_def;
 
@@ -61,7 +62,7 @@ val birs_pcond = (snd o dest_eq o concl) aes_bsysprecond_thm;
 val timer = bir_miscLib.timer_start 0;
 
 val result = bir_symb_analysis bprog_tm
- birs_state_init_lbl birs_stop_lbls
+ birs_state_init_lbl birs_state_end_lbls
  bprog_envtyl birs_pcond;
 
 val _ = bir_miscLib.timer_stop (fn delta_s => print ("\n======\n > bir_symb_analysis took " ^ delta_s ^ "\n")) timer;
