examples/riscv/swap/swap_propScript.sml
@@ -51,10 +51,11 @@ val riscv_cont_swap_thm =
   bir_swap_riscv_lift_THM;
 
 Theorem riscv_cont_swap:
- riscv_cont bir_swap_progbin 0x00w {0x14w}
+ riscv_cont bir_swap_progbin swap_init_addr {swap_end_addr}
   (riscv_swap_pre pre_x10 pre_x11 pre_x10_mem_deref pre_x11_mem_deref)
   (riscv_swap_post pre_x10 pre_x11 pre_x10_mem_deref pre_x11_mem_deref)
 Proof
+ rw [swap_init_addr_def,swap_end_addr_def] >>
  ACCEPT_TAC riscv_cont_swap_thm
 QED
 
