examples/riscv/swap/swap_symb_transfScript.sml
@@ -49,10 +49,30 @@ open swap_symb_execTheory;
 
 val _ = new_theory "swap_symb_transf";
 
+(* --------------------- *)
+(* Auxiliary definitions *)
+(* --------------------- *)
+
 val birs_state_ss = rewrites (type_rws ``:birs_state_t``);
+
+val bprog_tm = (fst o dest_eq o concl) bir_swap_prog_def;
+
+val init_addr_tm = (snd o dest_eq o concl) swap_init_addr_def;
+val end_addr_tm = (snd o dest_eq o concl) swap_end_addr_def;
 
 val bspec_swap_pre = ``bspec_swap_pre``;
 val bspec_swap_post = ``bspec_swap_post``;
+
+val birs_state_init_lbl = (snd o dest_eq o concl o EVAL)
+ ``bir_block_pc (BL_Address (Imm64 ^init_addr_tm))``;
+val birs_state_end_lbl = (snd o dest_eq o concl o EVAL)
+ ``bir_block_pc (BL_Address (Imm64 ^end_addr_tm))``;
+
+val birs_state_init_pre =  ``birs_state_init_pre_GEN
+ ^birs_state_init_lbl swap_birenvtyl
+ (mk_bsysprecond
+  (bspec_swap_pre pre_x10 pre_x11 pre_x10_mem_deref pre_x11_mem_deref)
+  swap_birenvtyl)``;
 
 (* ------------------------------- *)
 (* BIR symbolic execution analysis *)
@@ -64,14 +84,6 @@ Definition swap_analysis_L_def:
  swap_analysis_L = ^(L_s)
 End
 
-val init_addr_tm = (snd o dest_eq o concl) swap_init_addr_def;
-val end_addr_tm = (snd o dest_eq o concl) swap_end_addr_def;
-
-val birs_state_init_lbl = (snd o dest_eq o concl o EVAL)
- ``bir_block_pc (BL_Address (Imm64 ^init_addr_tm))``;
-val birs_state_end_lbl = (snd o dest_eq o concl o EVAL)
- ``bir_block_pc (BL_Address (Imm64 ^end_addr_tm))``;
-
 Theorem swap_analysis_L_NOTIN_thm[local]:
   (^birs_state_end_lbl) NOTIN swap_analysis_L
 Proof
@@ -82,10 +94,7 @@ QED
 (* ........................... *)
 (* ........................... *)
 
-val birs_state_init_pre = ``birs_state_init_pre_GEN ^birs_state_init_lbl swap_birenvtyl
- (mk_bsysprecond (bspec_swap_pre pre_x10 pre_x11 pre_x10_mem_deref pre_x11_mem_deref) swap_birenvtyl)``;
-
-Theorem birs_state_init_pre_EQ_thm:
+Theorem birs_state_init_pre_EQ_thm[local]:
   ^((snd o dest_comb) sys_i) = ^birs_state_init_pre
 Proof
   REWRITE_TAC [birs_state_init_pre_GEN_def, mk_bsysprecond_def, swap_bsysprecond_thm] >>
@@ -95,7 +104,7 @@ QED
 val swap_analysis_thm =
   REWRITE_RULE [birs_state_init_pre_EQ_thm, GSYM bir_swap_prog_def] swap_symb_analysis_thm;
 
-Theorem swap_birenvtyl_EVAL_thm =
+Theorem swap_birenvtyl_EVAL_thm[local] =
  (REWRITE_CONV [swap_birenvtyl_def,
    bir_lifting_machinesTheory.riscv_bmr_vars_EVAL,
    bir_lifting_machinesTheory.riscv_bmr_temp_vars_EVAL] THENC EVAL)
@@ -106,8 +115,6 @@ val birs_state_thm = REWRITE_CONV [swap_birenvtyl_EVAL_thm] birs_state_init_pre;
 (* ------ *)
 
 (* now the transfer *)
-
-val bprog_tm = (fst o dest_eq o concl) bir_swap_prog_def;
 
 val birs_symb_symbols_f_sound_prog_thm =
   (SPEC (inst [Type`:'observation_type` |-> Type.alpha] bprog_tm) bir_symb_soundTheory.birs_symb_symbols_f_sound_thm);
@@ -298,7 +305,7 @@ Theorem bir_abstract_jgmt_rel_swap_thm[local] =
 (* ........................... *)
 (* ........................... *)
 
-Theorem abstract_jgmt_rel_swap:
+Theorem abstract_jgmt_rel_swap[local]:
  abstract_jgmt_rel (bir_ts ^bprog_tm)
   (BL_Address (Imm64 ^init_addr_tm)) {BL_Address (Imm64 ^end_addr_tm)}
   (\st. bir_exec_to_labels_triple_precond st
@@ -308,7 +315,8 @@ Theorem abstract_jgmt_rel_swap:
          then (bspec_swap_post pre_x10 pre_x11 pre_x10_mem_deref pre_x11_mem_deref)
          else bir_exp_false) ^bprog_tm)
 Proof
-  MATCH_MP_TAC (REWRITE_RULE [boolTheory.AND_IMP_INTRO] abstract_jgmt_rel_bir_exec_to_labels_triple_thm) >>
+  MATCH_MP_TAC (REWRITE_RULE
+   [boolTheory.AND_IMP_INTRO] abstract_jgmt_rel_bir_exec_to_labels_triple_thm) >>
   SIMP_TAC std_ss [] >>
   Q.EXISTS_TAC `swap_birenvtyl` >>
   
@@ -348,12 +356,12 @@ Proof
   METIS_TAC [bir_abstract_jgmt_rel_swap_thm, pre_bir_nL_def, post_bir_nL_def, swap_prog_vars_thm]
 QED
 
-Theorem bspec_cont_swap_tm[local]:
+Theorem bspec_cont_swap_thm[local]:
  bir_cont ^bprog_tm bir_exp_true
   (BL_Address (Imm64 ^init_addr_tm)) {BL_Address (Imm64 ^end_addr_tm)} {}
   (bspec_swap_pre pre_x10 pre_x11 pre_x10_mem_deref pre_x11_mem_deref)
   (\l. if l = BL_Address (Imm64 ^end_addr_tm)
-       then (bspec_swap_post pre_x10 pre_x11 pre_x10_mem_deref pre_x11_mem_deref)
+       then bspec_swap_post pre_x10 pre_x11 pre_x10_mem_deref pre_x11_mem_deref
        else bir_exp_false)
 Proof
  `{BL_Address (Imm64 ^end_addr_tm)} <> {}` by fs [] >>
@@ -364,20 +372,21 @@ Proof
   `\l. if l = BL_Address (Imm64 ^end_addr_tm)
        then (bspec_swap_post pre_x10 pre_x11 pre_x10_mem_deref pre_x11_mem_deref)
        else bir_exp_false`
- ] o SPEC bprog_tm o INST_TYPE [Type.alpha |-> Type`:'observation_type`]) abstract_jgmt_rel_bir_cont) >>
+ ] o SPEC bprog_tm o INST_TYPE [Type.alpha |-> Type`:'observation_type`])
+   abstract_jgmt_rel_bir_cont) >>
  rw [] >>
  METIS_TAC [abstract_jgmt_rel_swap]
 QED
 
 Theorem bspec_cont_swap:
  bir_cont bir_swap_prog bir_exp_true
- (BL_Address (Imm64 ^init_addr_tm)) {BL_Address (Imm64 ^end_addr_tm)} {}
- (bspec_swap_pre pre_x10 pre_x11 pre_x10_mem_deref pre_x11_mem_deref)
+  (BL_Address (Imm64 ^init_addr_tm)) {BL_Address (Imm64 ^end_addr_tm)} {}
+  (bspec_swap_pre pre_x10 pre_x11 pre_x10_mem_deref pre_x11_mem_deref)
   (\l. if l = BL_Address (Imm64 ^end_addr_tm)
-       then (bspec_swap_post pre_x10 pre_x11 pre_x10_mem_deref pre_x11_mem_deref)
+       then bspec_swap_post pre_x10 pre_x11 pre_x10_mem_deref pre_x11_mem_deref
        else bir_exp_false)
 Proof
- rw [bir_swap_prog_def,bspec_cont_swap_tm]
+ rw [bir_swap_prog_def,bspec_cont_swap_thm]
 QED
 
 val _ = export_theory ();
